src/Pyrosome/Tools/PosRenaming.v
@@ -1,0 +1,111 @@
+(* TODO: largely duped from Int63Renaming. Adapt to a generic abstracion. *)
+Set Implicit Arguments.
+
+Require Import Lists.List NArith.
+Import ListNotations.
+Open Scope list.
+Open Scope positive.
+
+
+From coqutil Require Import Map.Interface.
+
+From Utils Require Import Utils Monad TrieMap.
+Import StateMonad.
+From Pyrosome Require Import Theory.Core.
+
+Section WithVar.
+  Context (V : Type)
+    {V_Eqb : Eqb V}
+    {V_default : WithDefault V}.
+  
+  Notation named_list := (@named_list V).
+  Notation named_map := (@named_map V).
+  Notation term := (@term V).
+  Notation ctx := (@ctx V).
+  Notation sort := (@sort V).
+  Notation subst := (@subst V).
+  Notation rule := (@rule V).
+  Notation lang := (@lang V).
+
+  Record renaming :=
+    MkRenaming {
+        p_to_v : trie_map V
+      ; v_to_p : named_list positive
+      ; next_id : positive
+      }.
+
+  
+  Definition empty_rename : renaming :=
+    MkRenaming map.empty [] 1.
+  
+
+  Local Notation ST := (state renaming).
+
+  Definition alloc (n : V) : ST positive :=
+    fun r =>
+      (r.(next_id),
+        MkRenaming (map.put r.(p_to_v) r.(next_id) n)
+          ((n,r.(next_id))::r.(v_to_p))
+          (Pos.add r.(next_id) 1)).
+
+  Definition to_p (v : V) : ST positive :=
+    fun r =>
+      match named_list_lookup_err r.(v_to_p) v with
+      | Some p => (p,r)
+      | None => alloc v r
+      end.
+
+  Fixpoint rename_term (e : term) : ST (Term.term positive) :=
+    match e with
+    | var x =>
+        @! let x' <- to_p x in
+          ret var x'
+    | con n s =>
+        @! let s' <- list_Mmap rename_term s in
+          let n' <- to_p n in
+          ret con n' s'
+    end.
+
+  Definition rename_sort (t : sort) : ST _ :=
+    let (n,s) := t in
+    @! let s' <- list_Mmap rename_term s in
+      let n' <- to_p n in
+      ret scon n' s'.
+
+  Definition rename_ctx (c : ctx) : ST _ :=
+    list_Mmap (fun '(x,t) =>
+                 @! let t' <- rename_sort t in
+                   let x' <- to_p x in
+                   ret (x',t')) c.
+  
+  Definition rename_rule r : ST _ :=
+    match r with
+    | sort_rule c args =>
+        @! let c' <- rename_ctx c in
+          let args' <- list_Mmap to_p args in
+          ret sort_rule c' args'
+    | term_rule c args t =>
+        @! let c' <- rename_ctx c in
+          let args' <- list_Mmap to_p args in
+          let t' <- rename_sort t in
+          ret term_rule c' args' t'
+    | sort_eq_rule c t1 t2 =>
+        @! let c' <- rename_ctx c in
+          let t1' <- rename_sort t1 in
+          let t2' <- rename_sort t2 in
+          ret sort_eq_rule c' t1' t2'
+    | term_eq_rule c e1 e2 t =>
+        @! let c' <- rename_ctx c in
+          let e1' <- rename_term e1 in
+          let e2' <- rename_term e2 in
+          let t' <- rename_sort t in
+          ret term_eq_rule c' e1' e2' t'
+    end.
+
+  Definition rename_lang : lang -> ST _ :=
+    list_Mmap (fun '(x,r) =>
+                 @! let r' <- rename_rule r in
+                   let x' <- to_p x in
+                   ret (x',r')).
+          
+End WithVar.
